*** empty log message ***

doc-src/TutorialI/Inductive/AB.thy
@@ -2,122 +2,307 @@
 
 section{*A context free grammar*}
 
+text{*
+Grammars are nothing but shorthands for inductive definitions of nonterminals
+which represent sets of strings. For example, the production
+$A \to B c$ is short for
+\[ w \in B \Longrightarrow wc \in A \]
+This section demonstrates this idea with a standard example
+\cite[p.\ 81]{HopcroftUllman}, a grammar for generating all words with an
+equal number of $a$'s and $b$'s:
+\begin{eqnarray}
+S &\to& \epsilon \mid b A \mid a B \nonumber\\
+A &\to& a S \mid b A A \nonumber\\
+B &\to& b S \mid a B B \nonumber
+\end{eqnarray}
+At the end we say a few words about the relationship of the formalization
+and the text in the book~\cite[p.\ 81]{HopcroftUllman}.
+
+We start by fixing the alpgabet, which consists only of @{term a}'s
+and @{term b}'s:
+*}
+
 datatype alfa = a | b;
 
-lemma [simp]: "(x ~= a) = (x = b) & (x ~= b) = (x = a)";
+text{*\noindent
+For convenience we includ the following easy lemmas as simplification rules:
+*}
+
+lemma [simp]: "(x \<noteq> a) = (x = b) \<and> (x \<noteq> b) = (x = a)";
 apply(case_tac x);
 by(auto);
+
+text{*\noindent
+Words over this alphabet are of type @{typ"alfa list"}, and
+the three nonterminals are declare as sets of such words:
+*}
 
 consts S :: "alfa list set"
        A :: "alfa list set"
        B :: "alfa list set";
 
+text{*\noindent
+The above productions are recast as a \emph{simultaneous} inductive
+definition of @{term S}, @{term A} and @{term B}:
+*}
+
 inductive S A B
 intros
-"[] : S"
-"w : A ==> b#w : S"
-"w : B ==> a#w : S"
+  "[] \<in> S"
+  "w \<in> A \<Longrightarrow> b#w \<in> S"
+  "w \<in> B \<Longrightarrow> a#w \<in> S"
 
-"w : S ==> a#w : A"
-"[| v:A; w:A |] ==> b#v@w : A"
+  "w \<in> S        \<Longrightarrow> a#w   \<in> A"
+  "\<lbrakk> v\<in>A; w\<in>A \<rbrakk> \<Longrightarrow> b#v@w \<in> A"
 
-"w : S ==> b#w : B"
-"[| v:B; w:B |] ==> a#v@w : B";
+  "w \<in> S            \<Longrightarrow> b#w   \<in> B"
+  "\<lbrakk> v \<in> B; w \<in> B \<rbrakk> \<Longrightarrow> a#v@w \<in> B";
 
-thm S_A_B.induct[no_vars];
+text{*\noindent
+First we show that all words in @{term S} contain the same number of @{term
+a}'s and @{term b}'s. Since the definition of @{term S} is by simultaneous
+induction, so is this proof: we show at the same time that all words in
+@{term A} contain one more @{term a} than @{term b} and all words in @{term
+B} contains one more @{term b} than @{term a}.
+*}
 
-lemma "(w : S --> size[x:w. x=a] = size[x:w. x=b]) &
-       (w : A --> size[x:w. x=a] = size[x:w. x=b] + 1) &
-       (w : B --> size[x:w. x=b] = size[x:w. x=a] + 1)";
+lemma correctness:
+  "(w \<in> S \<longrightarrow> size[x\<in>w. x=a] = size[x\<in>w. x=b])     \<and>
+    (w \<in> A \<longrightarrow> size[x\<in>w. x=a] = size[x\<in>w. x=b] + 1) \<and>
+    (w \<in> B \<longrightarrow> size[x\<in>w. x=b] = size[x\<in>w. x=a] + 1)"
+
+txt{*\noindent
+These propositions are expressed with the help of the predefined @{term
+filter} function on lists, which has the convenient syntax @{term"[x\<in>xs. P
+x]"}, the list of all elements @{term x} in @{term xs} such that @{prop"P x"}
+holds. The length of a list is usually written @{term length}, and @{term
+size} is merely a shorthand.
+
+The proof itself is by rule induction and afterwards automatic:
+*}
+
 apply(rule S_A_B.induct);
 by(auto);
 
-lemma intermed_val[rule_format(no_asm)]:
- "(!i<n. abs(f(i+1) - f i) <= #1) --> 
-  f 0 <= k & k <= f n --> (? i <= n. f i = (k::int))";
-apply(induct n);
- apply(simp);
- apply(arith);
-apply(rule);
-apply(erule impE);
- apply(simp);
-apply(rule);
-apply(erule_tac x = n in allE);
-apply(simp);
-apply(case_tac "k = f(n+1)");
- apply(force);
-apply(erule impE);
- apply(simp add:zabs_def split:split_if_asm);
- apply(arith);
-by(blast intro:le_SucI);
+text{*\noindent
+This may seem surprising at first, and is indeed an indication of the power
+of inductive definitions. But it is also quite straightforward. For example,
+consider the production $A \to b A A$: if $v,w \in A$ and the elements of $A$
+contain one more $a$ than $b$'s, then $bvw$ must again contain one more $a$
+than $b$'s.
 
-lemma step1: "ALL i < size w.
-  abs((int(size[x:take (i+1) w . P x]) - int(size[x:take (i+1) w . ~P x])) -
-      (int(size[x:take i w . P x]) - int(size[x:take i w . ~P x]))) <= #1";
+As usual, the correctness of syntactic descriptions is easy, but completeness
+is hard: does @{term S} contain \emph{all} words with an equal number of
+@{term a}'s and @{term b}'s? It turns out that this proof requires the
+following little lemma: every string with two more @{term a}'s than @{term
+b}'s can be cut somehwere such that each half has one more @{term a} than
+@{term b}. This is best seen by imagining counting the difference between the
+number of @{term a}'s than @{term b}'s starting at the left end of the
+word. We start at 0 and end (at the right end) with 2. Since each move to the
+right increases or decreases the difference by 1, we must have passed through
+1 on our way from 0 to 2. Formally, we appeal to the following discrete
+intermediate value theorem @{thm[source]nat0_intermed_int_val}
+@{thm[display]nat0_intermed_int_val[no_vars]}
+where @{term f} is of type @{typ"nat \<Rightarrow> int"}, @{typ int} are the integers,
+@{term abs} is the absolute value function, and @{term"#1::int"} is the
+integer 1 (see \S\ref{sec:int}).
+
+First we show that the our specific function, the difference between the
+numbers of @{term a}'s and @{term b}'s, does indeed only change by 1 in every
+move to the right. At this point we also start generalizing from @{term a}'s
+and @{term b}'s to an arbitrary property @{term P}. Otherwise we would have
+to prove the desired lemma twice, once as stated above and once with the
+roles of @{term a}'s and @{term b}'s interchanged.
+*}
+
+lemma step1: "\<forall>i < size w.
+  abs((int(size[x\<in>take (i+1) w.  P x]) -
+       int(size[x\<in>take (i+1) w. \<not>P x]))
+      -
+      (int(size[x\<in>take i w.  P x]) -
+       int(size[x\<in>take i w. \<not>P x]))) <= #1";
+
+txt{*\noindent
+The lemma is a bit hard to read because of the coercion function
+@{term[source]"int::nat \<Rightarrow> int"}. It is required because @{term size} returns
+a natural number, but @{text-} on @{typ nat} will do the wrong thing.
+Function @{term take} is predefined and @{term"take i xs"} is the prefix of
+length @{term i} of @{term xs}; below we als need @{term"drop i xs"}, which
+is what remains after that prefix has been dropped from @{term xs}.
+
+The proof is by induction on @{term w}, with a trivial base case, and a not
+so trivial induction step. Since it is essentially just arithmetic, we do not
+discuss it.
+*}
+
 apply(induct w);
  apply(simp);
-apply(simp add:take_Cons split:nat.split);
-apply(clarsimp);
-apply(rule conjI);
- apply(clarify);
- apply(erule allE);
- apply(erule impE);
-  apply(assumption);
- apply(arith);
-apply(clarify);
-apply(erule allE);
-apply(erule impE);
- apply(assumption);
-by(arith);
+by(force simp add:zabs_def take_Cons split:nat.split if_splits); 
 
+text{*
+Finally we come to the above mentioned lemma about cutting a word with two
+more elements of one sort than of the other sort into two halfs:
+*}
 
 lemma part1:
- "size[x:w. P x] = Suc(Suc(size[x:w. ~P x])) ==>
-  EX i<=size w. size[x:take i w. P x] = size[x:take i w. ~P x]+1";
-apply(insert intermed_val[OF step1, of "P" "w" "#1"]);
-apply(simp);
-apply(erule exE);
-apply(rule_tac x=i in exI);
-apply(simp);
-apply(rule int_int_eq[THEN iffD1]);
-apply(simp);
-by(arith);
+ "size[x\<in>w. P x] = size[x\<in>w. \<not>P x]+2 \<Longrightarrow>
+  \<exists>i\<le>size w. size[x\<in>take i w. P x] = size[x\<in>take i w. \<not>P x]+1";
+
+txt{*\noindent
+This is proved with the help of the intermediate value theorem, instantiated
+appropriately and with its first premise disposed of by lemma
+@{thm[source]step1}.
+*}
+
+apply(insert nat0_intermed_int_val[OF step1, of "P" "w" "#1"]);
+apply simp;
+by(simp del:int_Suc add:zdiff_eq_eq sym[OF int_Suc]);
+
+text{*\noindent
+The additional lemmas are needed to mediate between @{typ nat} and @{typ int}.
+
+Lemma @{thm[source]part1} tells us only about the prefix @{term"take i w"}.
+The suffix @{term"drop i w"} is dealt with in the following easy lemma:
+*}
+
 
 lemma part2:
-"[| size[x:take i xs @ drop i xs. P x] = size[x:take i xs @ drop i xs. ~P x]+2;
-    size[x:take i xs. P x] = size[x:take i xs. ~P x]+1 |]
- ==> size[x:drop i xs. P x] = size[x:drop i xs. ~P x]+1";
+  "\<lbrakk>size[x\<in>take i w @ drop i w. P x] =
+    size[x\<in>take i w @ drop i w. \<not>P x]+2;
+    size[x\<in>take i w. P x] = size[x\<in>take i w. \<not>P x]+1\<rbrakk>
+   \<Longrightarrow> size[x\<in>drop i w. P x] = size[x\<in>drop i w. \<not>P x]+1";
 by(simp del:append_take_drop_id);
 
-lemmas [simp] = S_A_B.intros;
+text{*\noindent
+Lemma @{thm[source]append_take_drop_id}, @{thm append_take_drop_id[no_vars]},
+which is generally useful, needs to be disabled for once.
 
-lemma "(size[x:w. x=a] = size[x:w. x=b] --> w : S) &
-       (size[x:w. x=a] = size[x:w. x=b] + 1 --> w : A) &
-       (size[x:w. x=b] = size[x:w. x=a] + 1 --> w : B)";
+To dispose of trivial cases automatically, the rules of the inductive
+definition are declared simplification rules:
+*}
+
+declare S_A_B.intros[simp];
+
+text{*\noindent
+This could have been done earlier but was not necessary so far.
+
+The completeness theorem tells us that if a word has the same number of
+@{term a}'s and @{term b}'s, then it is in @{term S}, and similarly and
+simultaneously for @{term A} and @{term B}:
+*}
+
+theorem completeness:
+  "(size[x\<in>w. x=a] = size[x\<in>w. x=b]     \<longrightarrow> w \<in> S) \<and>
+    (size[x\<in>w. x=a] = size[x\<in>w. x=b] + 1 \<longrightarrow> w \<in> A) \<and>
+    (size[x\<in>w. x=b] = size[x\<in>w. x=a] + 1 \<longrightarrow> w \<in> B)";
+
+txt{*\noindent
+The proof is by induction on @{term w}. Structural induction would fail here
+because, as we can see from the grammar, we need to make bigger steps than
+merely appending a single letter at the front. Hence we induct on the length
+of @{term w}, using the induction rule @{thm[source]length_induct}:
+*}
+
 apply(induct_tac w rule: length_induct);
-apply(case_tac "xs");
- apply(simp);
-apply(simp);
+(*<*)apply(rename_tac w)(*>*)
+
+txt{*\noindent
+The @{text rule} parameter tells @{text induct_tac} explicitly which induction
+rule to use. For details see \S\ref{sec:complete-ind} below.
+In this case the result is that we may assume the lemma already
+holds for all words shorter than @{term w}.
+
+The proof continues with a case distinction on @{term w},
+i.e.\ if @{term w} is empty or not.
+*}
+
+apply(case_tac w);
+ apply(simp_all);
+(*<*)apply(rename_tac x v)(*>*)
+
+txt{*\noindent
+Simplification disposes of the base case and leaves only two step
+cases to be proved:
+if @{prop"w = a#v"} and @{prop"size[x\<in>v. x=a] = size[x\<in>v. x=b]+2"} then
+@{prop"b#v \<in> A"}, and similarly for @{prop"w = b#v"}.
+We only consider the first case in detail.
+
+After breaking the conjuction up into two cases, we can apply
+@{thm[source]part1} to the assumption that @{term w} contains two more @{term
+a}'s than @{term b}'s.
+*}
+
 apply(rule conjI);
  apply(clarify);
- apply(frule part1[of "%x. x=a", simplified]);
+ apply(frule part1[of "\<lambda>x. x=a", simplified]);
  apply(erule exE);
  apply(erule conjE);
- apply(drule part2[of "%x. x=a", simplified]);
+
+txt{*\noindent
+This yields an index @{prop"i \<le> length v"} such that
+@{prop"length [x\<in>take i v . x = a] = length [x\<in>take i v . x = b] + 1"}.
+With the help of @{thm[source]part1} it follows that
+@{prop"length [x\<in>drop i v . x = a] = length [x\<in>drop i v . x = b] + 1"}.
+*}
+
+ apply(drule part2[of "\<lambda>x. x=a", simplified]);
   apply(assumption);
- apply(rule_tac n1=i and t=list in subst[OF append_take_drop_id]);
+
+txt{*\noindent
+Now it is time to decompose @{term v} in the conclusion @{prop"b#v \<in> A"}
+into @{term"take i v @ drop i v"},
+after which the appropriate rule of the grammar reduces the goal
+to the two subgoals @{prop"take i v \<in> A"} and @{prop"drop i v \<in> A"}:
+*}
+
+ apply(rule_tac n1=i and t=v in subst[OF append_take_drop_id]);
  apply(rule S_A_B.intros);
-  apply(force simp add:min_less_iff_disj);
+
+txt{*\noindent
+Both subgoals follow from the induction hypothesis because both @{term"take i
+v"} and @{term"drop i v"} are shorter than @{term w}:
+*}
+
+  apply(force simp add: min_less_iff_disj);
  apply(force split add: nat_diff_split);
+
+txt{*\noindent
+Note that the variables @{term n1} and @{term t} referred to in the
+substitution step above come from the derived theorem @{text"subst[OF
+append_take_drop_id]"}.
+
+The case @{prop"w = b#v"} is proved completely analogously:
+*}
+
 apply(clarify);
-apply(frule part1[of "%x. x=b", simplified]);
+apply(frule part1[of "\<lambda>x. x=b", simplified]);
 apply(erule exE);
 apply(erule conjE);
-apply(drule part2[of "%x. x=b", simplified]);
+apply(drule part2[of "\<lambda>x. x=b", simplified]);
  apply(assumption);
-apply(rule_tac n1=i and t=list in subst[OF append_take_drop_id]);
+apply(rule_tac n1=i and t=v in subst[OF append_take_drop_id]);
 apply(rule S_A_B.intros);
  apply(force simp add:min_less_iff_disj);
 by(force simp add:min_less_iff_disj split add: nat_diff_split);
+
+text{*
+We conclude this section with a comparison of the above proof and the one
+in the textbook \cite[p.\ 81]{HopcroftUllman}. For a start, the texbook
+grammar, for no good reason, excludes the empty word, which complicates
+matters just a little bit because we now have 8 instead of our 7 productions.
+
+More importantly, the proof itself is different: rather than separating the
+two directions, they perform one induction on the length of a word. This
+deprives them of the beauty of rule induction and in the easy direction
+(correctness) their reasoning is more detailed than our @{text auto}. For the
+hard part (completeness), they consider just one of the cases that our @{text
+simp_all} disposes of automatically. Then they conclude the proof by saying
+about the remaining cases: ``We do this in a manner similar to our method of
+proof for part (1); this part is left to the reader''. But this is precisely
+the part that requires the intermediate value theorem and thus is not at all
+similar to the other cases (which are automatic in Isabelle). We conclude
+that the authors are at least cavalier about this point and may even have
+overlooked the slight difficulty lurking in the omitted cases. This is not
+atypical for pen-and-paper proofs, once analysed in detail.  *}
 
 (*<*)end(*>*)
